prove more about provability
also but back equal and false in preformula,
also add more comments

language_term_n2.lean
@@ -1,16 +1,30 @@
+/- A development of first-order logic in Lean.
+
+* The object theory uses classical logic
+* We use de Bruijn variables.
+* We use a deep embedding of the logic, i.e. the type of terms and formulas is inductively defined.
+* There is no well-formedness predicate; all elements of type "term" are well-formed.
+-/
+
+-- depend on mathlib
+--import data.list.basic
+
 namespace tactic
 namespace interactive
 meta def congr1 : tactic unit := congr_core
 end interactive
 end tactic
 
+open list
 namespace fol
 structure Language := 
-(relations : ℕ → Type) (functions : ℕ → Type) (equal : relations 2) (false : relations 0)
+(relations : ℕ → Type) (functions : ℕ → Type)
 section
 parameter {L : Language}
 
-/- preterm n is a partially applied term. if applied to n terms, it becomes a term -/
+/- preterm n is a partially applied term. if applied to n terms, it becomes a term.
+* Every element of preterm 0 is well typed. 
+* We use this encoding to avoid mutual or nested inductive types, since those are not too convenient to work with in Lean. -/
 inductive preterm : ℕ → Type 
 | var : ℕ → preterm 0
 | func : ∀ {n : nat}, L.functions n → preterm n
@@ -18,44 +32,46 @@ inductive preterm : ℕ → Type
 open preterm
 @[reducible] def term := preterm 0
 
-local prefix `&`:max := var
+prefix `&`:max := _root_.fol.preterm.var
 
 /- lift_term_at _ t n m raises variables in t which are at least m by n -/
 @[simp] def lift_term_at : ∀ {l}, preterm l → ℕ → ℕ → preterm l
-| _ (var k)       n m := if m ≤ k then var (k+n) else var k
+| _ &k            n m := if m ≤ k then &(k+n) else &k
 | _ (func f)      n m := func f
 | _ (apply t1 t2) n m := apply (lift_term_at t1 n m) (lift_term_at t2 n m)
 
-local notation t ` ↑ `:55 n ` # `:55 m:55 := lift_term_at t n m
+notation t ` ↑ `:100 n ` # `:100 m:100 := _root_.fol.lift_term_at t n m -- input ↑ with \upa
 
 def lift_term (t : term) (n : ℕ) : term := t ↑ n # 0
 def lift_term1 (t : term) : term := t ↑ 1 # 0
 
+infix ` ↑↑ `:100 := _root_.fol.lift_term -- input ↑ with \upa
+postfix ` ↑1`:100 := _root_.fol.lift_term1 -- input ↑ with \upa
+
 lemma lift_term_at_inj : ∀ {l} {t t' : preterm l} {n m : ℕ}, t ↑ n # m = t' ↑ n # m → t = t'
-| _ (var k) (var k')          n m h := 
-  by by_cases h₁ : m ≤ k; by_cases h₂ : m ≤ k'; simp [h₁, h₂] at h; congr; 
-       [exact add_right_cancel h, skip, skip, assumption]; exfalso; 
-       try {apply h₁}; try {apply h₂}; subst h; 
-       apply le_trans (by assumption) (nat.le_add_right _ _)
-| _ (var k) (func f')         n m h := by by_cases h' : m ≤ k; simp [h'] at h; contradiction
-| _ (var k) (apply t1' t2')   n m h := by by_cases h' : m ≤ k; simp [h'] at h; contradiction
-| _ (func f) (var k')         n m h := by by_cases h' : m ≤ k'; simp [h'] at h; contradiction
+| _ &k &k' n m h := 
+  by by_cases h₁ : m ≤ k; by_cases h₂ : m ≤ k'; simp [h₁, h₂] at h; 
+     congr;[exact add_right_cancel h, skip, skip, assumption]; exfalso; try {apply h₁}; 
+     try {apply h₂}; subst h; apply le_trans (by assumption) (nat.le_add_right _ _)
+| _ &k (func f')              n m h := by by_cases h' : m ≤ k; simp [h'] at h; contradiction
+| _ &k (apply t1' t2')        n m h := by by_cases h' : m ≤ k; simp [h'] at h; contradiction
+| _ (func f) &k'              n m h := by by_cases h' : m ≤ k'; simp [h'] at h; contradiction
 | _ (func f) (func f')        n m h := h
 | _ (func f) (apply t1' t2')  n m h := by cases h
-| _ (apply t1 t2) (var k')    n m h := by by_cases h' : m ≤ k'; simp [h'] at h; contradiction
+| _ (apply t1 t2) &k'         n m h := by by_cases h' : m ≤ k'; simp [h'] at h; contradiction
 | _ (apply t1 t2) (func f')   n m h := by cases h
 | _ (apply t1 t2) (apply t1' t2') n m h := 
   begin injection h, congr; apply lift_term_at_inj; assumption end
 
 @[simp] lemma lift_term_at_zero : ∀ {l} (t : preterm l) (m : ℕ), t ↑ 0 # m = t
-| _ (var k)     m := by simp
+| _ &k            m := by simp
 | _ (func f)      m := by refl
 | _ (apply t1 t2) m := by dsimp; congr; apply lift_term_at_zero
 
 /- the following lemmas simplify iterated lifts, depending on the size of m' -/
 lemma lift_term_at2_small : ∀ {l} (t : preterm l) (n n') {m m'}, m' ≤ m → 
   (t ↑ n # m) ↑ n' # m' = (t ↑ n' # m') ↑ n # (m + n')
-| _ (var k)       n n' m m' H := 
+| _ &k            n n' m m' H := 
   begin 
     by_cases h : m ≤ k,
     { have h₁ : m' ≤ k, from le_trans H h,
@@ -72,7 +88,7 @@ lemma lift_term_at2_small : ∀ {l} (t : preterm l) (n n') {m m'}, m' ≤ m →
 
 lemma lift_term_at2_medium : ∀ {l} (t : preterm l) (n n') {m m'}, m ≤ m' → m' ≤ m+n → 
   (t ↑ n # m) ↑ n' # m' = t ↑ (n+n') # m
-| _ (var k)       n n' m m' H₁ H₂ := 
+| _ &k            n n' m m' H₁ H₂ := 
   begin 
     by_cases h : m ≤ k,
     { have h₁ : m' ≤ k + n, from le_trans H₂ (add_le_add_right h n),
@@ -90,55 +106,69 @@ lemma lift_term_at2_eq {l} (t : preterm l) (n n' m : ℕ) :
 lift_term_at2_medium t n n' (m.le_add_right n) (le_refl _)
 
 lemma lift_term_at2_large {l} (t : preterm l) (n n') {m m'} (H : m' ≥ m + n) : 
-  (t ↑ n # m) ↑ n' # m' = (t ↑ n' # m'-n) ↑ n # m :=
+  (t ↑ n # m) ↑ n' # m' = (t ↑ n' # (m'-n)) ↑ n # m :=
 have H₁ : n ≤ m', from le_trans (n.le_add_left m) H,
 have H₂ : m ≤ m' - n, by rw [←nat.add_sub_cancel m n]; apply nat.sub_le_sub_right; exact H,
 begin rw fol.lift_term_at2_small t n' n H₂, rw [nat.sub_add_cancel], exact H₁ end
 
-/- substitute_term t s n substitutes s for (var n) and reduces the level of all variables above n by 1 -/
+/- substitute_term t s n substitutes s for (&n) and reduces the level of all variables above n by 1 -/
 @[simp] def substitute_term : ∀ {l}, preterm l → term → ℕ → preterm l
-| _ (var k)     s n := if k < n then var k else if n < k then var (k-1) else s
+| _ &k            s n := if k < n then &k else if n < k then &(k-1) else s
 | _ (func f)      s n := func f
 | _ (apply t1 t2) s n := apply (substitute_term t1 s n) (substitute_term t2 s n)
 
-@[simp] def substitute_term_var_eq (t : term) (n : ℕ) : substitute_term &n t n = t :=
+notation t `[`:95 s ` // `:95 n `]`:0 := _root_.fol.substitute_term t s n
+
+@[simp] def substitute_term_var_eq (t : term) (n : ℕ) : &n[t // n] = t :=
 by simp [lt_irrefl]
 
-lemma substitute_term_lift_term' : ∀{l} (t : preterm l) (s : term), 
-  substitute_term (lift_term_at t 1 0) s 0 = t :=
+lemma substitute_term_lift_term' : ∀{l} (t : preterm l) (s : term) (n : ℕ), 
+  (lift_term_at t 1 n)[s // n] = t :=
 sorry
 
-@[simp] lemma substitute_term_lift_term (t s : term) : substitute_term (lift_term1 t) s 0 = t :=
-substitute_term_lift_term' t s
+@[simp] lemma substitute_term_lift_term (t s : term) : (lift_term1 t)[s // 0] = t :=
+substitute_term_lift_term' t s 0
 
-/- preformula n is a partially applied formula. if applied to n terms, it becomes a formula -/
+/- preformula n is a partially applied formula. if applied to n terms, it becomes a formula. 
+  * We only have implication as binary connective. Since we use classical logic, we can define
+    the other connectives from implication and false. 
+  * Similarly, universal quantification is our only quantifier. 
+  * We could make `false` and `equal` into elements of rel. However, if we do that, then we cannot make the interpretation of them in a model definitionally what we want.
+
+-/
 inductive preformula : ℕ → Type 
+| false : preformula 0
+| equal : term → term → preformula 0
 | rel : ∀ {n : nat}, L.relations n → preformula n
 | apprel : ∀ {n : nat}, preformula (n + 1) → term → preformula n
 | imp : preformula 0 → preformula 0 → preformula 0
 | all : preformula 0 → preformula 0
 open preformula
-def formula := preformula 0
+@[reducible] def formula := preformula 0
 
-def equal (t₁ t₂ : term) : formula := apprel (apprel (rel L.equal) t₁) t₂
-def false : formula := rel L.false
 def not (f : formula) : formula := imp f false
-def or (f₁ f₂ : formula) : formula := imp (not f₁) f₂
 def and (f₁ f₂ : formula) : formula := not (imp f₁ (not f₂))
+def or (f₁ f₂ : formula) : formula := imp (not f₁) f₂
 def iff (f₁ f₂ : formula) : formula := and (imp f₁ f₂) (imp f₂ f₁)
 def ex (f : formula) : formula := not (all (not f))
 
-local infix ` ⟾ `:70 := imp
-local infix ` ⇔ `:75 := iff
-local infix ` ≍ `:80 := equal
+notation `⊥` := _root_.fol.preformula.false -- input: \bot
+infix ` ≃ `:90 := _root_.fol.preformula.equal -- input \~- or \simeq
+infix ` ⟹ `:70 := _root_.fol.preformula.imp -- input \==>
+prefix `~` := _root_.fol.not
+infixr ` ⊔ `:80 := _root_.fol.or -- input: \sqcup
+infixr ` ⊓ `:85 := _root_.fol.and -- input: \sqcap
+
 
 @[simp] def lift_formula_at : ∀ {l}, preformula l → ℕ → ℕ → preformula l
+| _ false        n m := false
+| _ (t1 ≃ t2)    n m := equal (lift_term_at t1 n m) (lift_term_at t2 n m)
 | _ (rel R)      n m := rel R
 | _ (apprel f t) n m := apprel (lift_formula_at f n m) (lift_term_at t n m)
 | _ (imp f1 f2)  n m := imp (lift_formula_at f1 n m) (lift_formula_at f2 n m)
 | _ (all f)      n m := all (lift_formula_at f n (m+1))
 
-local notation f ` ↑ `:55 n ` # `:55 m:55 := lift_formula_at f n m
+notation f ` ↑ `:100 n ` # `:100 m:100 := _root_.fol.lift_formula_at f n m -- input ↑ with \upa
 
 def lift_formula (f : formula) (n : ℕ) : formula := f ↑ n # 0
 def lift_formula1 (f : formula) : formula := f ↑ 1 # 0
@@ -146,12 +176,15 @@ def lift_formula1 (f : formula) : formula := f ↑ 1 # 0
 lemma lift_formula_at_inj {l} {f f' : preformula l} {n m : ℕ} (H : f ↑ n # m = f' ↑ n # m) : f = f' :=
 begin
   induction f generalizing m; cases f'; injection H,
+  simp [lift_term_at_inj h_1, lift_term_at_inj h_2],
   simp [f_ih h_1, fol.lift_term_at_inj h_2],
   simp [f_ih_a h_1, f_ih_a_1 h_2],
   simp [f_ih h_1]
 end
 
 @[simp] lemma lift_formula_at_zero : ∀ {l} (f : preformula l) (m : ℕ), f ↑ 0 # m = f
+| _ false        m := by refl
+| _ (t1 ≃ t2)    m := by simp
 | _ (rel R)      m := by refl
 | _ (apprel f t) m := by simp; apply lift_formula_at_zero
 | _ (imp f1 f2)  m := by dsimp; congr1; apply lift_formula_at_zero
@@ -160,6 +193,8 @@ end
 /- the following lemmas simplify iterated lifts, depending on the size of m' -/
 lemma lift_formula_at2_small : ∀ {l} (f : preformula l) (n n') {m m'}, m' ≤ m → 
   (f ↑ n # m) ↑ n' # m' = (f ↑ n' # m') ↑ n # (m + n')
+| _ false        n n' m m' H := by refl
+| _ (t1 ≃ t2)    n n' m m' H := by simp [lift_term_at2_small, H]
 | _ (rel R)      n n' m m' H := by refl
 | _ (apprel f t) n n' m m' H := 
   by simp [lift_term_at2_small, H, -add_comm]; apply lift_formula_at2_small; assumption
@@ -169,6 +204,8 @@ lemma lift_formula_at2_small : ∀ {l} (f : preformula l) (n n') {m m'}, m' ≤ 
 
 lemma lift_formula_at2_medium : ∀ {l} (f : preformula l) (n n') {m m'}, m ≤ m' → m' ≤ m+n → 
   (f ↑ n # m) ↑ n' # m' = f ↑ (n+n') # m
+| _ false        n n' m m' H₁ H₂ := by refl
+| _ (t1 ≃ t2)    n n' m m' H₁ H₂ := by simp [lift_term_at2_medium, H₁, H₂]
 | _ (rel R)      n n' m m' H₁ H₂ := by refl
 | _ (apprel f t) n n' m m' H₁ H₂ :=
   by simp [lift_term_at2_medium, H₁, H₂, -add_comm]; apply lift_formula_at2_medium; assumption
@@ -182,55 +219,145 @@ lemma lift_formula_at2_eq {l} (f : preformula l) (n n' m : ℕ) :
 lift_formula_at2_medium f n n' (m.le_add_right n) (le_refl _)
 
 lemma lift_formula_at2_large {l} (f : preformula l) (n n') {m m'} (H : m' ≥ m + n) : 
-  (f ↑ n # m) ↑ n' # m' = (f ↑ n' # m'-n) ↑ n # m :=
+  (f ↑ n # m) ↑ n' # m' = (f ↑ n' # (m'-n)) ↑ n # m :=
 have H₁ : n ≤ m', from le_trans (n.le_add_left m) H,
 have H₂ : m ≤ m' - n, by rw [←nat.add_sub_cancel m n]; apply nat.sub_le_sub_right; exact H,
 begin rw fol.lift_formula_at2_small f n' n H₂, rw [nat.sub_add_cancel], exact H₁ end
 
 @[simp] def substitute_formula : ∀ {l}, preformula l → term → ℕ → preformula l
+| _ false        s n := false
+| _ (t1 ≃ t2)    s n := equal (substitute_term t1 s n) (substitute_term t2 s n)
 | _ (rel R)      s n := rel R
 | _ (apprel f t) s n := apprel (substitute_formula f s n) (substitute_term t s n)
 | _ (imp f1 f2)  s n := imp (substitute_formula f1 s n) (substitute_formula f2 s n)
 | _ (all f)      s n := all (substitute_formula f s (n+1))
 
-@[simp] def substitute_formula0 (f : formula) (t : term) := substitute_formula f t 0
+notation f `[`:95 s ` // `:95 n `]`:0 := _root_.fol.substitute_formula f s n
 
 @[simp] def substitute_formula_equal (t₁ t₂ s : term) (n : ℕ) :
-  substitute_formula (t₁ ≍ t₂) s n = substitute_term t₁ s n ≍ substitute_term t₂ s n :=
+  (t₁ ≃ t₂)[s // n] = t₁[s // n] ≃ (t₂[s // n]) :=
 by refl
 
--- ⟾⇔≍
-
+-- ⟹⇔≃
+/- Provability relation
+* to decide: should Γ be a list or a set (or finset)?
+* We use natural deduction as our deduction system, since that is most convenient to work with.
+* All rules are motivated to work well with backwards reasoning.
+-/
 inductive prf : list formula → formula → Type
 | axm    : ∀{Γ A}, A ∈ Γ → prf Γ A
-| impI   : ∀{Γ A B}, prf (A::Γ) B → prf Γ (A ⟾ B)
-| impE   : ∀{Γ A B}, prf Γ (A ⟾ B) → prf Γ A → prf Γ B
+| impI   : ∀{Γ A B}, prf (A::Γ) B → prf Γ (A ⟹ B)
+| impE   : ∀{Γ} (A) {B}, prf Γ (A ⟹ B) → prf Γ A → prf Γ B
 | falseE : ∀{Γ A}, prf (not A::Γ) false → prf Γ A
-| allI   : ∀{Γ A}, prf (list.map lift_formula1 Γ) A → prf Γ (all A)
-| allE   : ∀{Γ} A t, prf Γ (all A) → prf Γ (substitute_formula0 A t)
-| refl   : ∀Γ t, prf Γ (t ≍ t)
-| subst : ∀{Γ} s t f, prf Γ (s ≍ t) → prf Γ (substitute_formula f s 0) → 
-  prf Γ (substitute_formula f t 0)
+| allI   : ∀{Γ A}, prf (map lift_formula1 Γ) A → prf Γ (all A)
+| allE'  : ∀{Γ} A t, prf Γ (all A) → prf Γ (A[t // 0])
+| refl   : ∀Γ t, prf Γ (t ≃ t)
+| subst' : ∀{Γ} s t f, prf Γ (s ≃ t) → prf Γ (f[s // 0]) → prf Γ (f[t // 0])
 open prf
-local infix ` ⊢ `:51 := prf
+infix ` ⊢ `:51 := _root_.fol.prf -- input: \|- or \vdash
 
-def symm {Γ s t} (H : Γ ⊢ s ≍ t) : Γ ⊢ t ≍ s :=
-begin 
-  have H₁ := subst s t (equal (var 0) (lift_term1 s)) H, -- why does notation not work here?
-  rw [substitute_formula_equal, substitute_formula_equal, substitute_term_lift_term, substitute_term_lift_term, substitute_term_var_eq, substitute_term_var_eq] at H₁,
-  exact H₁ (refl Γ s)
+def weakening {Γ Δ} {f : formula} (H₁ : Γ ⊆ Δ) (H₂ : Γ ⊢ f) : Δ ⊢ f :=
+begin
+  induction H₂ generalizing Δ,
+  { apply axm, exact H₁ H₂_a, },
+  { apply impI, apply H₂_ih, simp [cons_subset_cons, H₁] },
+  { apply impE, apply H₂_ih_a, assumption, apply H₂_ih_a_1, assumption },
+  { apply falseE, apply H₂_ih, simp [cons_subset_cons, H₁] },
+  { apply allI, apply H₂_ih, sorry /-simp [cons_subset_cons, H₁]-/ },
+  { apply allE', apply H₂_ih, assumption },
+  { apply refl },
+  { apply subst', apply H₂_ih_a, assumption, apply H₂_ih_a_1, assumption },
 end
 
-def trans {Γ t₁ t₂ t₃} (H : Γ ⊢ t₁ ≍ t₂) (H' : Γ ⊢ t₂ ≍ t₃) : Γ ⊢ t₁ ≍ t₃ :=
+def weakening_cons {Γ} {f₁ f₂ : formula} (H : Γ ⊢ f₂) : f₁::Γ ⊢ f₂ :=
+weakening (Γ.subset_cons f₁) H
+
+def weakening_cons2 {Γ} {f₁ f₂ f₃ : formula} (H : f₁::Γ ⊢ f₂) : f₁::f₃::Γ ⊢ f₂ :=
+weakening (cons_subset_cons _ (Γ.subset_cons _)) H
+
+def allE {Γ} (A : formula) (t) {B} (H₁ : prf Γ (all A)) (H₂ : A[t // 0] = B) : prf Γ B :=
+by induction H₂; exact allE' A t H₁
+
+def subst {Γ} {s t} (f₁ : formula) {f₂} (H₁ : prf Γ (s ≃ t)) (H₂ : prf Γ (f₁[s // 0])) 
+  (H₃ : f₁[t // 0] = f₂) : prf Γ f₂ :=
+by induction H₃; exact subst' s t f₁ H₁ H₂
+
+def axm1 {Γ} {A : formula} : A::Γ ⊢ A := by apply axm; left; refl
+def axm2 {Γ} {A B : formula} : A::B::Γ ⊢ B := by apply axm; right; left; refl
+
+def deduction {Γ} {A B : formula} (H : Γ ⊢ A ⟹ B) : A::Γ ⊢ B :=
+impE A (weakening_cons H) axm1
+
+def exfalso {Γ} {A : formula} (H : prf Γ false) : prf Γ A :=
+falseE (weakening_cons H)
+
+def andI {Γ} {f₁ f₂ : formula} (H₁ : Γ ⊢ f₁) (H₂ : Γ ⊢ f₂) : Γ ⊢ f₁ ⊓ f₂ :=
 begin 
-  have H₁ := prf.subst t₂ t₃ (equal (lift_term1 t₁) (var 0)) H', 
-  rw [substitute_formula_equal, substitute_formula_equal, substitute_term_lift_term, substitute_term_lift_term, substitute_term_var_eq, substitute_term_var_eq] at H₁,
-  exact H₁ H
+  apply impI, apply impE f₂,
+  { apply impE f₁, apply axm1, exact weakening_cons H₁ },
+  { exact weakening_cons H₂ }
+end
+
+def andE1 {Γ f₁} (f₂ : formula) (H : Γ ⊢ f₁ ⊓ f₂) : Γ ⊢ f₁ :=
+begin 
+  apply falseE, apply impE _ (weakening_cons H), apply impI, apply exfalso,
+  apply impE f₁; [apply axm2, apply axm1]
+end
+
+def andE2 {Γ} (f₁ : formula) {f₂} (H : Γ ⊢ f₁ ⊓ f₂) : Γ ⊢ f₂ :=
+begin 
+  apply falseE, apply impE _ (weakening_cons H), apply impI, apply axm2
+end
+
+def orI1 {Γ} {A B : formula} (H : Γ ⊢ A) : Γ ⊢ A ⊔ B :=
+begin
+  apply impI, apply exfalso, refine impE _ _ (weakening_cons H), apply axm1
+end
+
+def orI2 {Γ} {A B : formula} (H : Γ ⊢ B) : Γ ⊢ A ⊔ B :=
+impI $ weakening_cons H
+
+def orE {Γ} {A B C : formula} (H₁ : Γ ⊢ A ⊔ B) (H₂ : A::Γ ⊢ C) (H₃ : B::Γ ⊢ C) : Γ ⊢ C :=
+begin
+  apply falseE, apply impE C, { apply axm1 },
+  apply impE B, { apply impI, exact weakening_cons2 H₃ },
+  apply impE _ (weakening_cons H₁),
+  apply impI (impE _ axm2 (weakening_cons2 H₂))
+end
+
+def iffI {Γ} {f₁ f₂ : formula} (H₁ : f₁::Γ ⊢ f₂) (H₂ : f₂::Γ ⊢ f₁) : Γ ⊢ iff f₁ f₂ :=
+by apply andI; apply impI; assumption
+
+def iffE1 {Γ} {f₁ f₂ : formula} (H : Γ ⊢ iff f₁ f₂) : f₁::Γ ⊢ f₂ :=
+deduction (andE1 _ H)
+
+def iffE2 {Γ} {f₁ f₂ : formula} (H : Γ ⊢ iff f₁ f₂) : f₂::Γ ⊢ f₁ :=
+deduction (andE2 _ H)
+
+-- def ex (f : formula) : formula := not (all (not f))
+
+def symm {Γ} {s t : term} (H : Γ ⊢ s ≃ t) : Γ ⊢ t ≃ s :=
+begin 
+  apply subst (&0 ≃ s ↑1) H; 
+    rw [substitute_formula_equal, substitute_term_lift_term, substitute_term_var_eq],
+  apply refl
+end
+
+def trans {Γ} {t₁ t₂ t₃ : term} (H : Γ ⊢ t₁ ≃ t₂) (H' : Γ ⊢ t₂ ≃ t₃) : Γ ⊢ t₁ ≃ t₃ :=
+begin 
+  apply subst (t₁ ↑1 ≃ &0) H';
+    rw [substitute_formula_equal, substitute_term_lift_term, substitute_term_var_eq],
+  exact H
+end
+
+def congr {Γ} {t₁ t₂ s : term} (H : Γ ⊢ t₁ ≃ t₂) : Γ ⊢ s[t₁ // 0] ≃ s[t₂ // 0] :=
+begin 
+  apply subst (s[t₁ // 0] ↑1 ≃ s) H, 
+  { rw [substitute_formula_equal, substitute_term_lift_term], apply refl },
+  { rw [substitute_formula_equal, substitute_term_lift_term] }
 end
 
 end
 end fol
 open fol fol.preterm
 variable {L : Language}
-#check substitute_formula0 (@equal L (var 0) (var 0)) (var 7)
-#reduce substitute_formula0 (@equal L (var 0) (var 0)) (var 7)
